Stated failing sim lemma.

HBSim.v
@@ -2571,7 +2571,7 @@ Proof.
 (* Do we want a failing iexec as well? *)
 
 Inductive fail_iexec P G t :
-  list operation -> list conc_op -> state -> env -> Prop :=
+  list operation -> list conc_op -> (*state -> env -> *)Prop :=
   | fail_raw P1 P2 a x o v1 v2 rest vs1 vs2
     (Hload: P=P1++(t, load_handler t x zt ++
                                    Load a (x, o) :: Unlock (X + x) :: rest) :: P2)
@@ -2579,8 +2579,8 @@ Inductive fail_iexec P G t :
       fail_iexec P G t (acq t (X + x) :: events_hb_check (W + x) (C + t) vs1 vs2 t )
                   (Acq t (X + x) ::
                    mops_hb_check (W + x) (C + t) vs1 vs2 zt t)
-        []
-        (upd_env (upd_env G t tmp1 v1) t tmp2 v2)
+        (*[]
+        (upd_env (upd_env G t tmp1 v1) t tmp2 v2)*)
   | fail_waw P1 P2 x o e v1 v2 rest vs1 vs2
       (Hstore : P = P1 ++ (t, store_handler t x zt ++
                               Store (x, o) e :: Unlock (X + x) :: rest) :: P2)
@@ -2588,8 +2588,8 @@ Inductive fail_iexec P G t :
       fail_iexec P G t (acq t (X + x) :: events_hb_check (W + x) (C + t) vs1 vs2 t )
                   (Acq t (X + x) ::
                    mops_hb_check (W + x) (C + t) vs1 vs2 zt t )
-        []
-        (upd_env (upd_env G t tmp1 v1) t tmp2 v2)
+        (*[]
+        (upd_env (upd_env G t tmp1 v1) t tmp2 v2)*)
   | fail_war P1 P2 x o e v1 v2 rest vs1 vs2 vs3
       (Hstore : P = P1 ++ (t, store_handler t x zt ++
                               Store (x, o) e :: Unlock (X + x) :: rest) :: P2)
@@ -2599,12 +2599,12 @@ Inductive fail_iexec P G t :
                   (Acq t (X + x) ::
                        mops_hb_check (W + x) (C + t) vs1 vs2 zt t ++
                   mops_hb_check (R+x) (C + t) vs3 vs2 zt t )
-        []
-        (upd_env (upd_env G t tmp1 v1) t tmp2 v2) 
+        (*[]
+        (upd_env (upd_env G t tmp1 v1) t tmp2 v2) *)
   | fail_assert P1 P2 e1 e2 rest
       (Hassert : P = P1 ++ (t, Assert_le e1 e2 :: rest) :: P2)
       (Hfail : eval (G t) e1 > eval (G t) e2) :
-      fail_iexec P G t [] [] [] G.
+      fail_iexec P G t [] [] (*[] G*).
 
 Lemma t_steps_length' : forall t P' G' li1 P G lo lc (Hdistinct : distinct P)
   (Ht_steps : t_steps P G t (length li1) lo lc (Some P') G')
@@ -7067,6 +7067,19 @@ Proof.
      exploit sim_step; eauto; clarify.
      eexists. split; eauto. 
 Qed.
+
+Lemma instrument_sim_race2 : forall (*P*) P1 P2 G1 G2 t (*h*)
+  (Hfresh : fresh_tmps P1) (Hlocs : safe_locs P1)
+  (Ht : Forall (fun e => fst e < zt) P1) (Hdistinct: distinct P2)
+  (HPsim : state_sim P1 P2) (HGsim : env_sim G1 G2)
+  m (*(Hroot : exec_star (Some (init_state P)) init_env h m (Some P1) G1)*)
+  (Hinit : forall p, meta_loc p -> initialized m p)
+  o2 c2 (Hstep : fail_iexec P2 G2 t o2 c2)
+  (Hcon : consistent (m ++ c2)) s (Hs : clocks_sim m s),
+  exists o c P1' G1', exec P1 G1 t o c (Some P1') G1' /\
+    forall s', ~step_star s (opt_to_list o) s'.
+Proof.
+Abort.
 
 Theorem instrument_correct : forall P h m P' G'
   (HP : exec_star (Some (init_state P)) init_env h m (Some P') G'),
